git-svn-id: https://projects.brucker.ch/hol-testgen/svn/HOL-TestGen/trunk/hol-testgen@10409 3260e6d1-4efc-4170-b0a7-36055960796d

src/OCL_lib.thy
@@ -143,47 +143,47 @@ technical reasons; these operators are heavily overloaded in the HOL library
 that a further overloading would lead to heavy technical buzz in this
 document.
 *}
-definition OclAdd\<^sub>I\<^sub>n\<^sub>t\<^sub>e\<^sub>g\<^sub>e\<^sub>r ::"('\<AA>)Integer \<Rightarrow> ('\<AA>)Integer \<Rightarrow> ('\<AA>)Integer" (infix "`+" 40)
-where "x `+ y \<equiv> \<lambda> \<tau>. if (\<delta> x) \<tau> = true \<tau> \<and> (\<delta> y) \<tau> = true \<tau>
+definition OclAdd\<^sub>I\<^sub>n\<^sub>t\<^sub>e\<^sub>g\<^sub>e\<^sub>r ::"('\<AA>)Integer \<Rightarrow> ('\<AA>)Integer \<Rightarrow> ('\<AA>)Integer" (infix "+\<^sub>o\<^sub>c\<^sub>l" 40)
+where "x +\<^sub>o\<^sub>c\<^sub>l y \<equiv> \<lambda> \<tau>. if (\<delta> x) \<tau> = true \<tau> \<and> (\<delta> y) \<tau> = true \<tau>
                 then \<lfloor>\<lfloor>\<lceil>\<lceil>x \<tau>\<rceil>\<rceil> + \<lceil>\<lceil>y \<tau>\<rceil>\<rceil>\<rfloor>\<rfloor>
                 else invalid \<tau> "
 
-definition OclLess\<^sub>I\<^sub>n\<^sub>t\<^sub>e\<^sub>g\<^sub>e\<^sub>r ::"('\<AA>)Integer \<Rightarrow> ('\<AA>)Integer \<Rightarrow> ('\<AA>)Boolean" (infix "`<" 40)
-where "x `< y \<equiv> \<lambda> \<tau>. if (\<delta> x) \<tau> = true \<tau> \<and> (\<delta> y) \<tau> = true \<tau>
+definition OclLess\<^sub>I\<^sub>n\<^sub>t\<^sub>e\<^sub>g\<^sub>e\<^sub>r ::"('\<AA>)Integer \<Rightarrow> ('\<AA>)Integer \<Rightarrow> ('\<AA>)Boolean" (infix "<\<^sub>o\<^sub>c\<^sub>l" 40)
+where "x <\<^sub>o\<^sub>c\<^sub>l y \<equiv> \<lambda> \<tau>. if (\<delta> x) \<tau> = true \<tau> \<and> (\<delta> y) \<tau> = true \<tau>
                 then \<lfloor>\<lfloor>\<lceil>\<lceil>x \<tau>\<rceil>\<rceil> < \<lceil>\<lceil>y \<tau>\<rceil>\<rceil>\<rfloor>\<rfloor>
                 else invalid \<tau> "
 
-definition OclLe\<^sub>I\<^sub>n\<^sub>t\<^sub>e\<^sub>g\<^sub>e\<^sub>r ::"('\<AA>)Integer \<Rightarrow> ('\<AA>)Integer \<Rightarrow> ('\<AA>)Boolean" (infix "`\<le>" 40)
-where "x `\<le> y \<equiv> \<lambda> \<tau>. if (\<delta> x) \<tau> = true \<tau> \<and> (\<delta> y) \<tau> = true \<tau>
+definition OclLe\<^sub>I\<^sub>n\<^sub>t\<^sub>e\<^sub>g\<^sub>e\<^sub>r ::"('\<AA>)Integer \<Rightarrow> ('\<AA>)Integer \<Rightarrow> ('\<AA>)Boolean" (infix "\<le>\<^sub>o\<^sub>c\<^sub>l" 40)
+where "x \<le>\<^sub>o\<^sub>c\<^sub>l y \<equiv> \<lambda> \<tau>. if (\<delta> x) \<tau> = true \<tau> \<and> (\<delta> y) \<tau> = true \<tau>
                 then \<lfloor>\<lfloor>\<lceil>\<lceil>x \<tau>\<rceil>\<rceil> \<le> \<lceil>\<lceil>y \<tau>\<rceil>\<rceil>\<rfloor>\<rfloor>
                 else invalid \<tau> "
 
 subsubsection{* Basic Properties *}
 
-lemma OclAdd\<^sub>I\<^sub>n\<^sub>t\<^sub>e\<^sub>g\<^sub>e\<^sub>r_commute: "(X `+ Y) = (Y `+ X)"
+lemma OclAdd\<^sub>I\<^sub>n\<^sub>t\<^sub>e\<^sub>g\<^sub>e\<^sub>r_commute: "(X +\<^sub>o\<^sub>c\<^sub>l Y) = (Y +\<^sub>o\<^sub>c\<^sub>l X)"
   by(rule ext,auto simp:true_def false_def OclAdd\<^sub>I\<^sub>n\<^sub>t\<^sub>e\<^sub>g\<^sub>e\<^sub>r_def invalid_def
                    split: option.split option.split_asm
                           bool.split bool.split_asm)
 
 subsubsection{* Execution with Invalid or Null or Zero as Argument *}
 
-lemma OclAdd\<^sub>I\<^sub>n\<^sub>t\<^sub>e\<^sub>g\<^sub>e\<^sub>r_strict1[simp,code_unfold] : "(x `+ invalid) = invalid"
+lemma OclAdd\<^sub>I\<^sub>n\<^sub>t\<^sub>e\<^sub>g\<^sub>e\<^sub>r_strict1[simp,code_unfold] : "(x +\<^sub>o\<^sub>c\<^sub>l invalid) = invalid"
 by(rule ext, simp add: OclAdd\<^sub>I\<^sub>n\<^sub>t\<^sub>e\<^sub>g\<^sub>e\<^sub>r_def true_def false_def)
 
-lemma OclAdd\<^sub>I\<^sub>n\<^sub>t\<^sub>e\<^sub>g\<^sub>e\<^sub>r_strict2[simp,code_unfold] : "(invalid `+ x) = invalid"
+lemma OclAdd\<^sub>I\<^sub>n\<^sub>t\<^sub>e\<^sub>g\<^sub>e\<^sub>r_strict2[simp,code_unfold] : "(invalid +\<^sub>o\<^sub>c\<^sub>l x) = invalid"
 by(rule ext, simp add: OclAdd\<^sub>I\<^sub>n\<^sub>t\<^sub>e\<^sub>g\<^sub>e\<^sub>r_def true_def false_def)
 
-lemma [simp,code_unfold] : "(x `+ null) = invalid"
+lemma [simp,code_unfold] : "(x +\<^sub>o\<^sub>c\<^sub>l null) = invalid"
 by(rule ext, simp add: OclAdd\<^sub>I\<^sub>n\<^sub>t\<^sub>e\<^sub>g\<^sub>e\<^sub>r_def true_def false_def)
 
-lemma [simp,code_unfold] : "(null `+ x) = invalid"
+lemma [simp,code_unfold] : "(null +\<^sub>o\<^sub>c\<^sub>l x) = invalid"
 by(rule ext, simp add: OclAdd\<^sub>I\<^sub>n\<^sub>t\<^sub>e\<^sub>g\<^sub>e\<^sub>r_def true_def false_def)
 
 lemma OclAdd\<^sub>I\<^sub>n\<^sub>t\<^sub>e\<^sub>g\<^sub>e\<^sub>r_zero1[simp,code_unfold] :
-"(x `+ \<zero>) = (if \<upsilon> x and not (\<delta> x) then invalid else x endif)"
+"(x +\<^sub>o\<^sub>c\<^sub>l \<zero>) = (if \<upsilon> x and not (\<delta> x) then invalid else x endif)"
  proof (rule ext, rename_tac \<tau>, case_tac "(\<upsilon> x and not (\<delta> x)) \<tau> = true \<tau>")
   fix \<tau> show "(\<upsilon> x and not (\<delta> x)) \<tau> = true \<tau> \<Longrightarrow>
-              (x `+ \<zero>) \<tau> = (if \<upsilon> x and not (\<delta> x) then invalid else x endif) \<tau>"
+              (x +\<^sub>o\<^sub>c\<^sub>l \<zero>) \<tau> = (if \<upsilon> x and not (\<delta> x) then invalid else x endif) \<tau>"
    apply(subst OclIf_true', simp add: OclValid_def)
   by (metis OclAdd\<^sub>I\<^sub>n\<^sub>t\<^sub>e\<^sub>g\<^sub>e\<^sub>r_def OclNot_defargs OclValid_def foundation5 foundation9)
   apply_end assumption
@@ -196,7 +196,7 @@ lemma OclAdd\<^sub>I\<^sub>n\<^sub>t\<^sub>e\<^sub>g\<^sub>e\<^sub>r_zero1[simp,
    apply(rename_tac x', case_tac x', metis bot_option_def foundation16 null_option_def)
   by(simp)
   show "\<tau> \<Turnstile> not (\<upsilon> x and not (\<delta> x)) \<Longrightarrow>
-              (x `+ \<zero>) \<tau> = (if \<upsilon> x and not (\<delta> x) then invalid else x endif) \<tau>"
+              (x +\<^sub>o\<^sub>c\<^sub>l \<zero>) \<tau> = (if \<upsilon> x and not (\<delta> x) then invalid else x endif) \<tau>"
    apply(subst OclIf_false', simp, simp add: A, auto simp: OclAdd\<^sub>I\<^sub>n\<^sub>t\<^sub>e\<^sub>g\<^sub>e\<^sub>r_def OclInt0_def)
      (* *)
      apply (metis OclValid_def foundation19 foundation20)
@@ -206,28 +206,28 @@ lemma OclAdd\<^sub>I\<^sub>n\<^sub>t\<^sub>e\<^sub>g\<^sub>e\<^sub>r_zero1[simp,
 qed
 
 lemma OclAdd\<^sub>I\<^sub>n\<^sub>t\<^sub>e\<^sub>g\<^sub>e\<^sub>r_zero2[simp,code_unfold] :
-"(\<zero> `+ x) = (if \<upsilon> x and not (\<delta> x) then invalid else x endif)"
+"(\<zero> +\<^sub>o\<^sub>c\<^sub>l x) = (if \<upsilon> x and not (\<delta> x) then invalid else x endif)"
 by(subst OclAdd\<^sub>I\<^sub>n\<^sub>t\<^sub>e\<^sub>g\<^sub>e\<^sub>r_commute, simp)
 
 subsubsection{* Context Passing *}
 
-lemma cp_OclAdd\<^sub>I\<^sub>n\<^sub>t\<^sub>e\<^sub>g\<^sub>e\<^sub>r:"(X `+ Y) \<tau> = ((\<lambda> _. X \<tau>) `+ (\<lambda> _. Y \<tau>)) \<tau>"
+lemma cp_OclAdd\<^sub>I\<^sub>n\<^sub>t\<^sub>e\<^sub>g\<^sub>e\<^sub>r:"(X +\<^sub>o\<^sub>c\<^sub>l Y) \<tau> = ((\<lambda> _. X \<tau>) +\<^sub>o\<^sub>c\<^sub>l (\<lambda> _. Y \<tau>)) \<tau>"
 by(simp add: OclAdd\<^sub>I\<^sub>n\<^sub>t\<^sub>e\<^sub>g\<^sub>e\<^sub>r_def cp_defined[symmetric])
 
-lemma cp_OclLess\<^sub>I\<^sub>n\<^sub>t\<^sub>e\<^sub>g\<^sub>e\<^sub>r:"(X `< Y) \<tau> = ((\<lambda> _. X \<tau>) `< (\<lambda> _. Y \<tau>)) \<tau>"
+lemma cp_OclLess\<^sub>I\<^sub>n\<^sub>t\<^sub>e\<^sub>g\<^sub>e\<^sub>r:"(X <\<^sub>o\<^sub>c\<^sub>l Y) \<tau> = ((\<lambda> _. X \<tau>) <\<^sub>o\<^sub>c\<^sub>l (\<lambda> _. Y \<tau>)) \<tau>"
 by(simp add: OclLess\<^sub>I\<^sub>n\<^sub>t\<^sub>e\<^sub>g\<^sub>e\<^sub>r_def cp_defined[symmetric])
 
-lemma cp_OclLe\<^sub>I\<^sub>n\<^sub>t\<^sub>e\<^sub>g\<^sub>e\<^sub>r:"(X `\<le> Y) \<tau> = ((\<lambda> _. X \<tau>) `\<le> (\<lambda> _. Y \<tau>)) \<tau>"
+lemma cp_OclLe\<^sub>I\<^sub>n\<^sub>t\<^sub>e\<^sub>g\<^sub>e\<^sub>r:"(X \<le>\<^sub>o\<^sub>c\<^sub>l Y) \<tau> = ((\<lambda> _. X \<tau>) \<le>\<^sub>o\<^sub>c\<^sub>l (\<lambda> _. Y \<tau>)) \<tau>"
 by(simp add: OclLe\<^sub>I\<^sub>n\<^sub>t\<^sub>e\<^sub>g\<^sub>e\<^sub>r_def cp_defined[symmetric])
 
 subsubsection{* Test Statements *}
 text{* Here follows a list of code-examples, that explain the meanings
 of the above definitions by compilation to code and execution to @{term "True"}.*}
 
-Assert "  \<tau> \<Turnstile> ( \<nine> `\<le> \<one>\<zero> )"
-Assert "  \<tau> \<Turnstile> (( \<four> `+ \<four> ) `\<le> \<one>\<zero> )"
-Assert "\<not>(\<tau> \<Turnstile> (( \<four> `+ ( \<four> `+ \<four> )) `< \<one>\<zero> ))"
-Assert "  \<tau> \<Turnstile> not (\<upsilon> (null `+ \<one>)) "
+Assert "  \<tau> \<Turnstile> ( \<nine> \<le>\<^sub>o\<^sub>c\<^sub>l \<one>\<zero> )"
+Assert "  \<tau> \<Turnstile> (( \<four> +\<^sub>o\<^sub>c\<^sub>l \<four> ) \<le>\<^sub>o\<^sub>c\<^sub>l \<one>\<zero> )"
+Assert "\<not>(\<tau> \<Turnstile> (( \<four> +\<^sub>o\<^sub>c\<^sub>l ( \<four> +\<^sub>o\<^sub>c\<^sub>l \<four> )) <\<^sub>o\<^sub>c\<^sub>l \<one>\<zero> ))"
+Assert "  \<tau> \<Turnstile> not (\<upsilon> (null +\<^sub>o\<^sub>c\<^sub>l \<one>)) "
 
 section{* Fundamental Predicates on Basic Types: Strict Equality *}
 
@@ -442,8 +442,8 @@ Assert "  \<tau> \<Turnstile> (\<four> \<doteq> \<four>)"
 Assert "\<not>(\<tau> \<Turnstile> (\<four> <> \<four>))"
 Assert "\<not>(\<tau> \<Turnstile> (\<four> \<doteq> \<one>\<zero>))"
 Assert "  \<tau> \<Turnstile> (\<four> <> \<one>\<zero>)"
-Assert "\<not>(\<tau> \<Turnstile> (\<zero> `< null))"
-Assert "\<not>(\<tau> \<Turnstile> (\<delta> (\<zero> `< null)))"
+Assert "\<not>(\<tau> \<Turnstile> (\<zero> <\<^sub>o\<^sub>c\<^sub>l null))"
+Assert "\<not>(\<tau> \<Turnstile> (\<delta> (\<zero> <\<^sub>o\<^sub>c\<^sub>l null)))"
 
 
 section{* Complex Types: The Set-Collection Type (I) Core *}
@@ -2253,7 +2253,7 @@ by(simp add: Abs_Set_0_inverse bot_option_def null_option_def OclInt0_def)
 
 lemma OclSize_including_exec[simp,code_unfold]:
  "((X ->including(x)) ->size()) = (if \<delta> X and \<upsilon> x then
-                                     X ->size() `+ if X ->includes(x) then \<zero> else \<one> endif
+                                     X ->size() +\<^sub>o\<^sub>c\<^sub>l if X ->includes(x) then \<zero> else \<one> endif
                                    else
                                      invalid
                                    endif)"
@@ -2289,7 +2289,7 @@ proof -
   by (metis (hide_lams, no_types) Set_inv_lemma foundation18' foundation5)
 
   show "X->including(x)->size() \<tau> = (if \<delta> X and \<upsilon> x
-                                     then X->size() `+ if X->includes(x) then \<zero> else \<one> endif
+                                     then X->size() +\<^sub>o\<^sub>c\<^sub>l if X->includes(x) then \<zero> else \<one> endif
                                      else invalid endif) \<tau>"
    apply(case_tac "\<tau> \<Turnstile> \<delta> X and \<upsilon> x", simp)
     apply(subst cp_OclAdd\<^sub>I\<^sub>n\<^sub>t\<^sub>e\<^sub>g\<^sub>e\<^sub>r)
@@ -3520,13 +3520,13 @@ Assert "\<not> (\<tau> \<Turnstile> (Set{\<two>,\<one>}->includes(null)))"
 Assert    "\<tau> \<Turnstile> (Set{\<two>,null}->includes(null))"
 Assert    "\<tau> \<Turnstile> (Set{null,\<two>}->includes(null))"
 
-Assert    "\<tau> \<Turnstile> ((Set{})->forAll(z | \<zero> `< z))"
+Assert    "\<tau> \<Turnstile> ((Set{})->forAll(z | \<zero> <\<^sub>o\<^sub>c\<^sub>l z))"
 
-Assert    "\<tau> \<Turnstile> ((Set{\<two>,\<one>})->forAll(z | \<zero> `< z))"
-Assert "\<not> (\<tau> \<Turnstile> ((Set{\<two>,\<one>})->exists(z | z `< \<zero> )))"
-Assert "\<not> (\<tau> \<Turnstile> \<delta>(Set{\<two>,null})->forAll(z | \<zero> `< z))"
-Assert "\<not> (\<tau> \<Turnstile> ((Set{\<two>,null})->forAll(z | \<zero> `< z)))"
-Assert    "\<tau> \<Turnstile> ((Set{\<two>,null})->exists(z | \<zero> `< z))"
+Assert    "\<tau> \<Turnstile> ((Set{\<two>,\<one>})->forAll(z | \<zero> <\<^sub>o\<^sub>c\<^sub>l z))"
+Assert "\<not> (\<tau> \<Turnstile> ((Set{\<two>,\<one>})->exists(z | z <\<^sub>o\<^sub>c\<^sub>l \<zero> )))"
+Assert "\<not> (\<tau> \<Turnstile> \<delta>(Set{\<two>,null})->forAll(z | \<zero> <\<^sub>o\<^sub>c\<^sub>l z))"
+Assert "\<not> (\<tau> \<Turnstile> ((Set{\<two>,null})->forAll(z | \<zero> <\<^sub>o\<^sub>c\<^sub>l z)))"
+Assert    "\<tau> \<Turnstile> ((Set{\<two>,null})->exists(z | \<zero> <\<^sub>o\<^sub>c\<^sub>l z))"
 
 Assert "\<not> (\<tau> \<Turnstile> (Set{null::'a Boolean} \<doteq> Set{}))"
 Assert "\<not> (\<tau> \<Turnstile> (Set{null::'a Integer} \<doteq> Set{}))"
